drop proofs

DNF/Theory/List.lean
@@ -1,136 +1,20 @@
 /- Copyright (c) Heather Macbeth, 2023.  All rights reserved. -/
-import Mathlib.Data.List.ProdSigma
+import Batteries.Data.List.Basic
+import Mathlib.Data.SProd
 
-@[ext] theorem BEq.ext {x y : BEq α} (h : x.beq = y.beq) : x = y := by
-  cases x
-  simp at h
-  rw [h]
+-- from `Mathlib.Data.List.Defs`
+instance instSProd : SProd (List α) (List β) (List (α × β)) where
+  sprod := List.product
 
-
-theorem beq_prod_diamond [DecidableEq α] [DecidableEq β] : instBEqOfDecidableEq (α := α × β) = instBEqProd := by
-  ext ⟨a1, b1⟩ ⟨a2, b2⟩
-  simp [instBEqProd, instBEqOfDecidableEq]
-
-theorem beq_list_diamond_aux [DecidableEq α] (l1 l2 : List α) : decide (l1 = l2) = List.beq l1 l2 := by
-  match l1, l2 with
-  | [], [] => rw [List.beq]; simp
-  | a::as, b::bs =>
-    rw [List.beq, ← beq_list_diamond_aux as bs]
-    simp only [List.cons.injEq, Bool.decide_and]
-    rfl
-  | _, _ => sorry
-
-theorem beq_list_diamond [DecidableEq α] : instBEqOfDecidableEq (α := List α) = List.instBEq := by
-  ext l1 l2
-  exact beq_list_diamond_aux l1 l2
+/-- `l.Forall p` is equivalent to `∀ a ∈ l, p a`, but unfolds directly to a conjunction, i.e.
+`List.Forall p [0, 1, 2] = p 0 ∧ p 1 ∧ p 2`. -/
+-- from `Mathlib.Data.List.Defs`
+@[simp]
+def List.Forall (p : α → Prop) : List α → Prop
+  | [] => True
+  | x :: [] => p x
+  | x :: l => p x ∧ Forall p l
 
 def List.Exists (p : α → Prop) : List α → Prop
   | [] => False
   | x :: l => p x ∨ Exists p l
-
-@[simp] theorem List.exists_nil (p : α → Prop) : ¬ [].Exists p := not_false
-
-@[simp] theorem List.exists_cons (p : α → Prop) (l : List α) (x : α) :
-    (x :: l).Exists p ↔ p x ∨ Exists p l :=
-  Iff.rfl
-
-@[simp] theorem List.exists_append (p : α → Prop) (l₁ l₂ : List α) :
-    (l₁ ++ l₂).Exists p ↔ l₁.Exists p ∨ l₂.Exists p := by
-  induction l₁ with
-  | nil => simp
-  | cons _ _ IH => simp [or_assoc, IH]
-
-theorem List.exists_iff_mem (p : α → Prop) (l : List α) :
-    l.Exists p ↔ ∃ x ∈ l, p x := by
-  induction l with
-  | nil => simp
-  | cons _ _ IH => simp [IH]
-
-@[simp] theorem List.not_exists (p : α → Prop) (l : List α) :
-    ¬ l.Exists p ↔ l.Forall (fun a ↦ ¬ p a) := by
-  simp [List.exists_iff_mem, List.forall_iff_forall_mem]
-
-@[simp] theorem List.not_forall (p : α → Prop) (l : List α) :
-    ¬ l.Forall p ↔ l.Exists (fun a ↦ ¬ p a) := by
-  simp [List.exists_iff_mem, List.forall_iff_forall_mem]
-
-theorem List.of_forall_of_mem {p : α → Prop} {l : List α} {x : α} (hx : x ∈ l) (hp : l.Forall p) :
-    p x := by
-  rw [List.forall_iff_forall_mem] at hp
-  exact hp x hx
-
-@[simp] theorem List.forall_append {l1 l2 : List α} :
-    (l1 ++ l2).Forall p ↔ l1.Forall p ∧ l2.Forall p := by
-  simp [List.forall_iff_forall_mem]
-  aesop
-
-theorem List.forall_of_forall_erase [DecidableEq α] {p : α → Prop} {l : List α} {x : α}
-    (hp : (l.erase x).Forall p) (hx : p x) :
-    l.Forall p := by
-  induction l with
-  | nil => simp
-  | cons head tail IH =>
-    rw [List.erase_cons] at hp
-    split at hp
-    next h =>
-      sorry
-      -- rw [h]
-      -- simp
-      -- exact ⟨hx, hp⟩
-    simp at hp ⊢
-    refine ⟨hp.1, IH hp.2⟩
-
-theorem List.find?_of_forall {l : List α} {q : α → Bool} (hq : l.find? q = some a) {P : α → Prop}
-    (hP : l.Forall P) :
-    P a := by
-  induction l with
-  | nil => simp at hq
-  | cons hd tl IH =>
-    rw [List.find?] at hq
-    simp only [forall_cons] at hP
-    split at hq
-    · simp only [Option.some.injEq] at hq
-      obtain rfl := hq
-      exact hP.1
-    · exact IH hq hP.2
-
-theorem List.mem_replace [BEq α] [LawfulBEq α] {l : List α} {a : α} (hal : a ∈ l) (b : α) :
-    b ∈ l.replace a b := by
-  induction l with
-  | nil => simp at hal
-  | cons head tail IH =>
-    rw [replace_cons]
-    split
-    next => simp
-    next h =>
-      simp at hal
-      obtain rfl | ha_tail := hal
-      · simp at h
-      right
-      exact IH ha_tail
-
-theorem List.forall_of_forall_replace [BEq α] [LawfulBEq α] {l : List α} {a : α}
-    {b : α} {P : α → Prop} (hPa : P a) (hPl : (l.replace a b).Forall P) :
-    l.Forall P := by
-  induction l with
-  | nil => simp
-  | cons head tail IH =>
-    rw [replace_cons] at hPl
-    simp at IH
-    split at hPl
-    next ha_head =>
-      simp at ha_head
-      subst ha_head
-      simp at hPl
-      simpa using ⟨hPa, hPl.2⟩
-    next =>
-      simp at hPl
-      simpa using ⟨hPl.1, IH hPl.2⟩
-
-theorem Option.elim_false {α : Type*} {p : Option α} {P : α → Prop} (h : Option.elim p False P) :
-    ∃ a, p = some a ∧ P a :=
-  match p with
-  | none => by simp at h
-  | some a => ⟨a, rfl, h⟩
-
-attribute [pp_dot] Option.elim
