DNF/Theory/ProveFalseFromSAT.lean
@@ -1,8 +1,5 @@
 /- Copyright (c) Heather Macbeth, 2023.  All rights reserved. -/
 import DNF.Theory.List
-import Mathlib.Tactic.ToExpr
-
-/-! ## SAT solver -/
 
 /-- A formula such as `P ∧ (Q ∨ (¬ P ∧ R))`, comprised of ∧, ∨, ¬ and some atoms indexed by a type
 `α`. -/
@@ -21,173 +18,16 @@ def insertAndDedup (p : α × Bool) : List (α × Bool) → Option (List (α × 
     (insertAndDedup p tl).elim none <| fun l =>
     (l.find? (fun p => p.1 == hd.1)).elim (hd :: l) fun p => if p.2 == hd.2 then l else none
 
-@[simp] theorem insertAndDedup_nil (p : α × Bool) : insertAndDedup p [] = some [p] := rfl
-
-theorem insertAndDedup_cons_of_none {p : α × Bool} {l : List (α × Bool)}
-    (hl : insertAndDedup p l = none) (hd : α × Bool) :
-    insertAndDedup p (hd :: l) = none := by
-  simp [insertAndDedup, hl]
-
-theorem insertAndDedup_cons {p : α × Bool} {l l' : List (α × Bool)}
-    (hl : insertAndDedup p l = some l') (hd : α × Bool) :
-    insertAndDedup p (hd :: l)
-    = (l'.find? (fun p => p.1 == hd.1)).elim (some (hd :: l'))
-      fun p => if p.2 == hd.2 then some l' else none := by
-  simp [insertAndDedup, hl]
-
-theorem insertAndDedup_none_of_cons_of_none {p : α × Bool} {c pl : List (α × Bool)} {hd : α × Bool}
-    (h : insertAndDedup p (hd :: c) = some pl) :
-    (hd ∈ pl ∧ insertAndDedup p c = some pl) ∨ ∃ l, pl = hd :: l ∧ insertAndDedup p c = some l := by
-  set iphd := insertAndDedup p c with h_iphd
-  clear_value iphd
-  cases iphd with
-  | none => simp [insertAndDedup_cons_of_none h_iphd.symm hd] at h
-  | some l =>
-    have H := insertAndDedup_cons h_iphd.symm hd
-    rw [H] at h
-    clear H
-    set search := l.find? (fun p ↦ p.1 == hd.1) with hp
-    clear_value search
-    cases search with
-    | none =>
-      simp at h
-      rw [←h]
-      right
-      use l
-    | some p' =>
-      have hp' := List.find?_some hp.symm
-      simp at h hp'
-      sorry
-      -- split at h
-      -- next hp'2 =>
-      --   left
-      --   rw [← Prod.ext hp' hp'2]
-      --   simp at h
-      --   rw [← h]
-      --   exact ⟨List.find?_mem hp.symm, rfl⟩
-      -- · simp at h
-
 def interpretBool (P : α → Prop) (p : α × Bool) : Prop := if p.2 then P p.1 else ¬ P p.1
-
-theorem not_interpretBool (P : α → Prop) (p : α × Bool) :
-    ¬ interpretBool P p ↔ interpretBool P (p.1, !p.2) := by
-  obtain ⟨a, bool⟩ := p
-  cases bool <;> simp [interpretBool]
-
-theorem List.forall_insertAndDedup {P : α → Prop} {p : α × Bool} (h1 : interpretBool P p)
-    {l : List (α × Bool)} (h2 : l.Forall (interpretBool P)) :
-    (insertAndDedup p l).elim False (List.Forall (interpretBool P)) := by
-  induction' l with head tail IH
-  · simpa
-  obtain ⟨hP_head, hP_tail⟩ :
-      interpretBool P head ∧ List.Forall (interpretBool P) tail := by
-    simpa only [List.forall_cons] using h2
-  obtain ⟨l, hs, IH⟩ := Option.elim_false (IH hP_tail)
-  rw [insertAndDedup_cons hs]
-  set a := l.find? (fun p ↦ p.1 == head.1) with ha
-  match a with
-  | none => simpa using ⟨hP_head, IH⟩
-  | some p' =>
-    rw [Option.elim_some]
-    have hp'_head : p'.1 = head.1 := by simpa using List.find?_some ha.symm
-    have hp'_P := List.find?_of_forall ha.symm IH
-    rw [interpretBool] at hp'_P hP_head
-    split at hp'_P
-    next hp' =>
-      rw [hp']
-      split at hP_head
-      next h_head =>
-        rw [h_head]
-        simpa using IH
-      next =>
-        rw [← hp'_head] at hP_head
-        contradiction
-    next hp' =>
-      simp at hp'
-      rw [hp']
-      split at hP_head
-      next =>
-        rw [← hp'_head] at hP_head
-        contradiction
-      next h_head =>
-        simp at h_head
-        rw [h_head]
-        simpa using IH
-
-theorem List.forall_of_forall_insertAndDedup {P : α → Prop} {p : α × Bool} {c l : List (α × Bool)}
-    (h1 : insertAndDedup p c = some l) (h2 : l.Forall (interpretBool P)) :
-    interpretBool P p ∧ c.Forall (interpretBool P) := by
-  induction c generalizing l with
-  | nil =>
-    simp at h1
-    subst h1
-    simpa
-  | cons head tail IH =>
-    obtain ⟨h_hd_l, hl⟩ | ⟨l', hl'⟩ := insertAndDedup_none_of_cons_of_none h1
-    · replace IH := IH hl h2
-      simp only [forall_cons]
-      exact ⟨IH.1, List.of_forall_of_mem h_hd_l h2, IH.2⟩
-    · rw [hl'.1] at h2
-      simp at h2
-      have H := IH hl'.2 h2.2
-      simp
-      refine ⟨H.1, h2.1, H.2⟩
 
 def combine : List (α × Bool) × List (α × Bool) → Option (List (α × Bool))
   | ([], l) => pure l
   | (hd :: tl, l) => (combine (tl, l)).bind <| insertAndDedup hd
 
-theorem List.forall_combine {P : α → Prop} {l1 l2 : List (α × Bool)}
-    (h1 : l1.Forall (interpretBool P)) (h2 : l2.Forall (interpretBool P)) :
-    (combine (l1, l2)).elim False (List.Forall (interpretBool P)) := by
-  induction l1 with
-  | nil => simpa [combine]
-  | cons head tail IH =>
-    simp at h1
-    obtain ⟨n, hn, hPn⟩ := Option.elim_false (IH h1.2)
-    rw [combine, hn, Option.some_bind]
-    exact List.forall_insertAndDedup h1.1 hPn
-
-theorem List.forall_of_forall_combine {P : α → Prop} {l : List (α × Bool)}
-    (hlP : l.Forall (interpretBool P)) {l₁ l₂ : List (α × Bool)} (hl : combine (l₁, l₂) = some l) :
-    l₁.Forall (interpretBool P) ∧ l₂.Forall (interpretBool P) := by
-  induction l₁ generalizing l with
-  | nil =>
-    have : some l₂ = some l := by
-      show pure l₂ = some _
-      simpa [combine] using hl
-    obtain rfl : l₂ = l := by simpa using this
-    simpa using hlP
-  | cons _ _ IH =>
-    simp [combine] at hl
-    obtain ⟨n, hn, hnl⟩ := hl
-    obtain ⟨hP, hPn⟩ := List.forall_of_forall_insertAndDedup hnl hlP
-    have H := IH hPn hn
-    simp
-    exact ⟨⟨hP, H.1⟩, H.2⟩
-
 def negate : List (List (α × Bool)) → List (List (α × Bool))
   | [] => [[]]
   | hd :: tl => hd ×ˢ (negate tl) |>.map
     (fun ((a, bool), l) => insertAndDedup (a, !bool) l) |>.reduceOption
-
-theorem forall_exists_not_interpretBool_iff_exists_forall_interpretBool_negate
-    (ors : List (List (α × Bool))) (P : α → Prop) :
-    ors.Forall (List.Exists (fun p => ¬interpretBool P p))
-    ↔ (negate ors).Exists (List.Forall (interpretBool P)) := by
-  induction ors with
-  | nil => simp [negate]
-  | cons head tail IH =>
-    simp only [negate, List.mem_cons, imp_false, List.forall_cons, IH, List.reduceOption]
-    simp only [not_interpretBool, List.exists_iff_mem, List.mem_filterMap, List.mem_map,
-      List.mem_product, Prod.exists (α := α × Bool), id_eq, exists_eq_right]
-    constructor
-    · rintro ⟨⟨q, hq, hqP⟩, ⟨ands, h_ands, hP_ands⟩⟩
-      obtain ⟨l, hl⟩ := Option.elim_false (List.forall_insertAndDedup hqP hP_ands)
-      exact ⟨l, ⟨q, ands, ⟨hq, h_ands⟩, hl.1⟩, hl.2⟩
-    · rintro ⟨l, ⟨q, ands, ⟨hq, h_ands⟩, h_ands_l⟩, hlP⟩
-      obtain ⟨H1, H2⟩ := List.forall_of_forall_insertAndDedup h_ands_l hlP
-      exact ⟨⟨q, hq, H1⟩, ⟨ands, h_ands, H2⟩⟩
 
 /-- Disjunctive normal form of a list of SAT formulas. -/
 def SAT.dnf : SAT α → List (List (α × Bool))
@@ -210,54 +50,10 @@ their negations. -/
 def interpretDNF (P : α → Prop) (ors : List (List (α × Bool))) : Prop :=
   ors.Exists <| List.Forall (interpretBool P)
 
-/-- A truth assignment to the atoms of a SAT formula makes it valid, if and only if that truth
-assignment makes the formula's disjunctive normal form valid. -/
-theorem SAT.interpret_iff_interpretDNF (s : SAT α) (P : α → Prop) :
-    interpret P s ↔ interpretDNF P s.dnf := by
-  induction s with
-  | atom a =>
-    simp [interpret, interpretDNF, SAT.dnf, interpretBool]
-  | not s hs =>
-    simpa [interpret, interpretDNF, SAT.dnf, hs] using
-      forall_exists_not_interpretBool_iff_exists_forall_interpretBool_negate s.dnf P
-  | and s₁ s₂ hs₁ hs₂ =>
-    rw [interpret, hs₁, hs₂, SAT.dnf]
-    simp [interpretDNF, List.exists_iff_mem, List.reduceOption]
-    constructor
-    · rintro ⟨⟨l₁, hl₁, hl₁P⟩, ⟨l₂, hl₂, hl₂P⟩⟩
-      obtain ⟨l, hl, H⟩ := Option.elim_false (List.forall_combine hl₁P hl₂P)
-      exact ⟨l, ⟨l₁, l₂, ⟨hl₁, hl₂⟩, hl⟩, H⟩
-    · rintro ⟨l, ⟨l₁, l₂, hls, hl⟩, hlP⟩
-      obtain ⟨hl₁P, hl₂P⟩ := List.forall_of_forall_combine hlP hl
-      exact ⟨⟨_, hls.1, hl₁P⟩, ⟨_, hls.2, hl₂P⟩⟩
-  | or s₁ s₂ hs₁ hs₂ =>
-    rw [interpret, hs₁, hs₂]
-    simp only [interpretDNF, SAT.dnf, List.exists_append]
-
 /-- Disjunctive normal form of a list of SAT formulas. -/
 def List.dnf : List (SAT α) → List (List (α × Bool))
   | [] => [[]]
   | hd :: tl => hd.dnf ×ˢ tl.dnf |>.map combine |>.reduceOption
-
-/-- A truth assignment to the atoms of a list of SAT formulas makes them valid, if and only if that
-truth assignment makes the list's disjunctive normal form valid. -/
-theorem List.interpret_iff_interpretDNF (l : List (SAT α)) (P : α → Prop) :
-    l.Forall (interpret P) ↔ interpretDNF P l.dnf := by
-  induction l with
-  | nil => simp [interpretDNF, dnf]
-  | cons head tail IH =>
-    simp [IH, interpretDNF, dnf, List.reduceOption, List.exists_iff_mem,
-      SAT.interpret_iff_interpretDNF]
-    constructor
-    · rintro ⟨⟨a, ha, haP⟩, ⟨b, hb, hbP⟩⟩
-      obtain ⟨l, hl, H⟩ := Option.elim_false (List.forall_combine haP hbP)
-      exact ⟨l, ⟨a, b, ⟨ha, hb⟩, hl⟩, H⟩
-    · rintro ⟨l, ⟨a, b, hls, hl⟩, hlP⟩
-      obtain ⟨haP, hbP⟩ := List.forall_of_forall_combine hlP hl
-      exact ⟨⟨_, hls.1, haP⟩, ⟨_, hls.2, hbP⟩⟩
-
-alias ⟨List.interpretDNF_of_interpret, List.interpret_of_interpretDNF⟩ :=
-  List.interpret_iff_interpretDNF
 
 /-- Compute a boolean from a list of SAT formulas which should be `true` if it is satisfiable (i.e.
 there is a truth assignment which makes them simultaneously true), and `false` if they are
@@ -268,8 +64,5 @@ def determineSAT (l : List (SAT α)) : Bool := !l.dnf.isEmpty
 `false`, then `False` can be proved from the list of formulas. -/
 theorem proveFalseFromSAT (l : List (SAT α)) (hl : determineSAT l = false) (P : α → Prop)
     (H : l.Forall (interpret P)) :
-    False := by
-  rw [determineSAT, Bool.not_eq_false', List.isEmpty_iff_eq_nil] at hl
-  simp [List.interpret_iff_interpretDNF, hl, interpretDNF] at H
-
-initialize Lean.registerTraceClass `Meta.tauto2
+    False :=
+  sorry
